simplify ctxdep

theories/gitree/greifiers.v
@@ -3,11 +3,15 @@ From iris.base_logic.lib Require Export invariants.
 From gitrees Require Import prelude.
 From gitrees.gitree Require Import core reify.
 
-
-Section greifiers.
+Section greifiers_generic.
   #[local] Open Scope type.
+  Context (a : is_ctx_dep).
+  Notation sReifier := (sReifier a).
+  Notation sReifier_ops := (sReifier_ops a).
+  Notation sReifier_state := (sReifier_state a).
+  Notation sReifier_re := (sReifier_re a).
 
-    (** Global reifiers: a collection of reifiers *)
+  (** Global reifiers: a collection of reifiers *)
   Inductive gReifiers : nat → Type :=
   | gReifiers_nil : gReifiers 0
   | gReifiers_cons {n} : sReifier → gReifiers n → gReifiers (S n)
@@ -18,10 +22,11 @@ Section greifiers.
   Proof.
     revert P Hcons.
     refine match v with gReifiers_nil => tt
-                      | gReifiers_cons sR v => λ P Hcons, Hcons sR v end.
+                   | gReifiers_cons sR v => λ P Hcons, Hcons sR v end.
   Defined.
 
-  #[global] Instance gReifiers_lookup_total : ∀ m, LookupTotal (fin m) sReifier (gReifiers m) :=
+  #[global] Instance gReifiers_lookup_total
+    : ∀ m, LookupTotal (fin m) sReifier (gReifiers m) :=
   fix go m i {struct i} := let _ : ∀ m, LookupTotal _ _ _ := @go in
   match i in fin m return gReifiers m → sReifier with
   | 0%fin => grs_S_inv (λ _, sReifier) (λ x _, x)
@@ -30,7 +35,7 @@ Section greifiers.
 
   Program Definition gReifiers_ops {n} (rs : gReifiers n) : opsInterp :=
     {| opid := { i : fin n & opid (sReifier_ops (rs !!! i)) };
-       opsInterp_lookup := λ iop, sReifier_ops (rs !!! projT1 iop) (projT2 iop)
+      opsInterp_lookup := λ iop, sReifier_ops (rs !!! projT1 iop) (projT2 iop)
     |}.
   Next Obligation.
     intros n rs.
@@ -65,14 +70,14 @@ Section greifiers.
   Fixpoint gState_rest {m} (i : fin m) : gReifiers m → oFunctor :=
     match i in fin m return gReifiers m → oFunctor with
     | 0%fin => grs_S_inv (λ _, oFunctor)
-                 (λ sR rs, gReifiers_state rs)
+                (λ sR rs, gReifiers_state rs)
     | FS j => grs_S_inv (λ _, oFunctor)
-                 (λ sR rs, sReifier_state sR * gState_rest j rs)%OF
+               (λ sR rs, sReifier_state sR * gState_rest j rs)%OF
     end.
 
   Lemma gState_decomp' {m} (i : fin m) (rs : gReifiers m) {X} `{!Cofe X} :
     gReifiers_state rs ♯ X ≃
-       ((sReifier_state (rs !!! i) ♯ X) * (gState_rest i rs ♯ X))%type.
+      ((sReifier_state (rs !!! i) ♯ X) * (gState_rest i rs ♯ X))%type.
   Proof.
     revert i. induction rs as [|n r rs]=>i.
     { inversion i. }
@@ -105,47 +110,98 @@ Section greifiers.
   Proof. rewrite ofe_iso_12. reflexivity. Qed.
   Lemma gState_recomp_decomp {m} (i : fin m) {rs : gReifiers m} {X} `{!Cofe X}
     (σ : sReifier_state (rs !!! i) ♯ X) rest fs :
-      gState_decomp i fs ≡ (σ, rest) →
-      gState_recomp rest σ ≡ fs.
+    gState_decomp i fs ≡ (σ, rest) →
+    gState_recomp rest σ ≡ fs.
   Proof.
     unfold gState_recomp. simpl.
     intros <-. rewrite ofe_iso_21//.
   Qed.
   Opaque gState_recomp gState_decomp.
 
-  Program Definition gReifiers_re {n} (rs : gReifiers n) {X} `{!Cofe X}
-    (op : opid (gReifiers_ops rs)) :
-    (Ins (gReifiers_ops rs op) ♯ X) * (gReifiers_state rs ♯ X) * ((Outs (gReifiers_ops rs op) ♯ X) -n> laterO X) -n>
-      optionO (laterO X * (gReifiers_state rs ♯ X))
+End greifiers_generic.
+
+Section greifiers.
+  #[local] Open Scope type.
+
+  Program Definition gReifiers_re_ctx_indep {n} (rs : gReifiers NotCtxDep n) {X} `{!Cofe X}
+    (op : opid (gReifiers_ops NotCtxDep rs)) :
+    (Ins (gReifiers_ops NotCtxDep rs op) ♯ X) * (gReifiers_state NotCtxDep rs ♯ X) -n>
+      optionO ((Outs (gReifiers_ops NotCtxDep rs op) ♯ X) * (gReifiers_state NotCtxDep rs ♯ X))
+    :=  λne xst,
+      let  i := projT1 op in
+      let op' := projT2 op in
+      let x := xst.1 in
+      let st := xst.2 in
+      let fs := gState_decomp NotCtxDep i st in
+      let σ := fs.1 in
+      let rest := fs.2 in
+      let rx := sReifier_re NotCtxDep (rs !!! i) op' (x, σ) in
+      optionO_map (prodO_map idfun (gState_recomp NotCtxDep rest)) rx.
+  Next Obligation. solve_proper_please. Qed.
+
+  Program Definition gReifiers_re_ctx_dep {n} (rs : gReifiers CtxDep n) {X} `{!Cofe X}
+    (op : opid (gReifiers_ops CtxDep rs)) :
+    (Ins (gReifiers_ops CtxDep rs op) ♯ X) * (gReifiers_state CtxDep rs ♯ X)
+    * ((Outs (gReifiers_ops CtxDep rs op) ♯ X) -n> laterO X) -n>
+      optionO (laterO X * (gReifiers_state CtxDep rs ♯ X))
     :=  λne xst,
       let  i := projT1 op in
       let op' := projT2 op in
       let a := xst.1.1 in
       let b := xst.1.2 in
       let c := xst.2 in
-      let fs := gState_decomp i b in
+      let fs := gState_decomp CtxDep i b in
       let σ := fs.1 in
       let rest := fs.2 in
-      let rx := sReifier_re (rs !!! i) op' (a, σ, c) in
-      optionO_map (prodO_map idfun (gState_recomp rest)) rx.
+      let rx := sReifier_re CtxDep (rs !!! i) op' (a, σ, c) in
+      optionO_map (prodO_map idfun (gState_recomp CtxDep rest)) rx.
   Next Obligation. solve_proper_please. Qed.
 
-  (** We can turn a collection of reifiers into a single reifier *)
-  Definition gReifiers_sReifier {n} (rs : gReifiers n) : sReifier :=
-    {| sReifier_ops := gReifiers_ops rs;
-       sReifier_state := gReifiers_state rs;
-       sReifier_re := @gReifiers_re n rs;
-    |}.
+  Program Definition gReifiers_re_type {n}
+    (a : is_ctx_dep) (rs : gReifiers a n) {X} `{!Cofe X}
+    (op : opid (gReifiers_ops a rs)) : ofe :=
+    match a with
+    | CtxDep =>
+        prodO (prodO (Ins (gReifiers_ops a rs op) ♯ X) (gReifiers_state a rs ♯ X))
+          (Outs (gReifiers_ops a rs op) ♯ X -n> laterO X) -n>
+          optionO (prodO (laterO X) (gReifiers_state a rs ♯ X))
+    | NotCtxDep =>
+        prodO (Ins (gReifiers_ops a rs op) ♯ X) (gReifiers_state a rs ♯ X) -n>
+          optionO (prodO (Outs (gReifiers_ops a rs op) ♯ X) (gReifiers_state a rs ♯ X))
+    end.
 
-  Lemma gReifiers_re_idx {n} (i : fin n) (rs : gReifiers n)
-    {X} `{!Cofe X} (op : opid (sReifier_ops (rs !!! i)))
-    (x : Ins (sReifier_ops _ op) ♯ X)
-    (σ : sReifier_state (rs !!! i) ♯ X)
-    (κ : (Outs (sReifier_ops (rs !!! i) op) ♯ X -n> laterO X))
-    (rest : gState_rest i rs ♯ X) :
-    gReifiers_re rs (existT i op) (x, gState_recomp rest σ, κ) ≡
-      optionO_map (prodO_map idfun (gState_recomp rest))
-      (sReifier_re (rs !!! i) op (x, σ, κ)).
+  Program Definition gReifiers_re {n} (a : is_ctx_dep) (rs : gReifiers a n)
+    {X} `{!Cofe X}
+    (op : opid (gReifiers_ops a rs)) :
+    @gReifiers_re_type n a rs X _ op.
+  Proof.
+    destruct a.
+    - apply gReifiers_re_ctx_dep.
+    - apply gReifiers_re_ctx_indep.
+  Defined.
+
+  (** We can turn a collection of reifiers into a single reifier *)
+  Program Definition gReifiers_sReifier {n} (a : is_ctx_dep) (rs : gReifiers a n)
+    : sReifier a :=
+    {| sReifier_ops := gReifiers_ops a rs;
+      sReifier_state := gReifiers_state a rs;
+      sReifier_re X _ op := _;
+    |}.
+  Next Obligation.
+    intros n [|] rs X ? op.
+    - apply (@gReifiers_re n CtxDep rs X _ op).
+    - apply (@gReifiers_re n NotCtxDep rs X _ op).
+  Defined.
+
+  Lemma gReifiers_re_idx_ctx_dep {n} (i : fin n) (rs : gReifiers CtxDep n)
+    {X} `{!Cofe X} (op : opid (sReifier_ops CtxDep (rs !!! i)))
+    (x : Ins (sReifier_ops CtxDep _ op) ♯ X)
+    (σ : sReifier_state CtxDep (rs !!! i) ♯ X)
+    (rest : gState_rest CtxDep i rs ♯ X)
+    (κ : (Outs (sReifier_ops CtxDep (rs !!! i) op) ♯ X -n> laterO X)) :
+    gReifiers_re CtxDep rs (existT i op) (x, gState_recomp CtxDep rest σ, κ) ≡
+      optionO_map (prodO_map idfun (gState_recomp CtxDep rest))
+      (sReifier_re CtxDep (rs !!! i) op (x, σ, κ)).
   Proof.
     unfold gReifiers_re. cbn-[prodO_map optionO_map].
     f_equiv; last repeat f_equiv.
@@ -156,54 +212,135 @@ Section greifiers.
     - rewrite gState_decomp_recomp//.
   Qed.
 
-  Class subReifier {n} (r : sReifier) (rs : gReifiers n) :=
+  Lemma gReifiers_re_idx_ctx_indep {n} (i : fin n) (rs : gReifiers NotCtxDep n)
+    {X} `{!Cofe X} (op : opid (sReifier_ops NotCtxDep (rs !!! i)))
+    (x : Ins (sReifier_ops NotCtxDep _ op) ♯ X)
+    (σ : sReifier_state NotCtxDep (rs !!! i) ♯ X)
+    (rest : gState_rest NotCtxDep i rs ♯ X) :
+    gReifiers_re NotCtxDep rs (existT i op) (x, gState_recomp NotCtxDep rest σ) ≡
+      optionO_map (prodO_map idfun (gState_recomp NotCtxDep rest))
+      (sReifier_re NotCtxDep (rs !!! i) op (x, σ)).
+  Proof.
+    unfold gReifiers_re. cbn-[prodO_map optionO_map].
+    f_equiv; last repeat f_equiv.
+    - eapply optionO_map_proper.
+      intros [x1 x2]; simpl. f_equiv.
+      f_equiv. f_equiv.
+      rewrite gState_decomp_recomp//.
+    - rewrite gState_decomp_recomp//.
+  Qed.
+
+  Program Definition gReifiers_re_idx_type {n} a (i : fin n) (rs : gReifiers a n)
+    {X} `{!Cofe X} (op : opid (sReifier_ops a (rs !!! i)))
+    (x : Ins (sReifier_ops a _ op) ♯ X)
+    (σ : sReifier_state a (rs !!! i) ♯ X)
+    (rest : gState_rest a i rs ♯ X) :
+    Type.
+  Proof.
+    destruct a.
+    - apply (∀ (κ : (Outs (sReifier_ops CtxDep (rs !!! i) op) ♯ X -n> laterO X)),
+               gReifiers_re CtxDep rs (existT i op) (x, gState_recomp CtxDep rest σ, κ) ≡
+                 optionO_map (prodO_map idfun (gState_recomp CtxDep rest))
+                 (sReifier_re CtxDep (rs !!! i) op (x, σ, κ))).
+    - apply (gReifiers_re NotCtxDep rs (existT i op) (x, gState_recomp NotCtxDep rest σ) ≡
+               optionO_map (prodO_map idfun (gState_recomp NotCtxDep rest))
+               (sReifier_re NotCtxDep (rs !!! i) op (x, σ))).
+  Defined.
+
+  Lemma gReifiers_re_idx {n} a (i : fin n) (rs : gReifiers a n)
+    {X} `{!Cofe X} (op : opid (sReifier_ops a (rs !!! i)))
+    (x : Ins (sReifier_ops a _ op) ♯ X)
+    (σ : sReifier_state a (rs !!! i) ♯ X)
+    (rest : gState_rest a i rs ♯ X) : gReifiers_re_idx_type a i rs op x σ rest.
+  Proof.
+    destruct a.
+    - intros κ. apply gReifiers_re_idx_ctx_dep.
+    - apply gReifiers_re_idx_ctx_indep.
+  Qed.
+
+  Program Definition sR_re_type {n}
+    {X} `{!Cofe X} (a : is_ctx_dep) (r : sReifier a) (rs : gReifiers a n)
+    (sR_idx : fin n)
+    (sR_ops : subEff (sReifier_ops a r) (sReifier_ops a (rs !!! sR_idx)))
+    (sR_state : sReifier_state a r ♯ X ≃ sReifier_state a (rs !!! sR_idx) ♯ X)
+    (m : nat) (op : opid (sReifier_ops a r)) : Type.
+  Proof.
+    destruct a.
+    - apply (∀ (x : Ins (sReifier_ops CtxDep r op) ♯ X)
+               (y : laterO X)
+               (s1 s2 : sReifier_state CtxDep r ♯ X)
+               (k : (Outs (sReifier_ops CtxDep r op) ♯ X -n> laterO X)),
+               sReifier_re CtxDep r op (x, s1, k) ≡{m}≡ Some (y, s2) →
+               sReifier_re CtxDep (rs !!! sR_idx) (subEff_opid op)
+                 (subEff_ins x, sR_state s1, k ◎ (subEff_outs ^-1)) ≡{m}≡
+                 Some (y, sR_state s2)).
+    - apply (∀ (x : Ins (sReifier_ops NotCtxDep _ op) ♯ X)
+               (y : Outs (sReifier_ops NotCtxDep _ op) ♯ X)
+               (s1 s2 : sReifier_state NotCtxDep r ♯ X),
+               sReifier_re NotCtxDep r op (x, s1) ≡{m}≡ Some (y, s2) →
+               sReifier_re NotCtxDep (rs !!! sR_idx) (subEff_opid op)
+                 (subEff_ins x, sR_state s1) ≡{m}≡
+                 Some (subEff_outs y, sR_state s2)).
+  Defined.
+
+  Class subReifier {n} {a : is_ctx_dep} (r : sReifier a) (rs : gReifiers a n) :=
     { sR_idx : fin n;
-      sR_ops :: subEff (sReifier_ops r) (sReifier_ops (rs !!! sR_idx));
+      sR_ops :: subEff (sReifier_ops a r) (sReifier_ops a (rs !!! sR_idx));
       sR_state {X} `{!Cofe X} :
-      sReifier_state r ♯ X ≃ sReifier_state (rs !!! sR_idx) ♯ X;
-      sR_re (m : nat) {X} `{!Cofe X} (op : opid (sReifier_ops r))
-        (x : Ins (sReifier_ops r op) ♯ X)
-        (y : laterO X)
-        (s1 s2 : sReifier_state r ♯ X)
-        (k : (Outs (sReifier_ops r op) ♯ X -n> laterO X)) :
-      sReifier_re r op (x, s1, k) ≡{m}≡ Some (y, s2) →
-      sReifier_re (rs !!! sR_idx) (subEff_opid op)
-        (subEff_ins x, sR_state s1, k ◎ (subEff_outs ^-1)) ≡{m}≡
-        Some (y, sR_state s2)
+      sReifier_state a r ♯ X ≃ sReifier_state a (rs !!! sR_idx) ♯ X;
+      sR_re (m : nat) {X} `{!Cofe X} (op : opid (sReifier_ops a r))
+      : sR_re_type a r rs sR_idx sR_ops (@sR_state X _) m op
     }.
 
-  #[global] Instance subReifier_here {n} (r : sReifier) (rs : gReifiers n) :
-    subReifier r (gReifiers_cons r rs).
+  #[global] Instance subReifier_here {n} {a : is_ctx_dep}
+    (r : sReifier a) (rs : gReifiers a n) :
+    subReifier r (gReifiers_cons a r rs).
   Proof.
     simple refine ({| sR_idx := 0%fin |}).
     - simpl. apply subEff_id.
     - simpl. intros. apply iso_ofe_refl.
-    - intros X ? op x y ? s1 s2 k HEQ; simpl.
-      unfold ofe_iso_1'; simpl.
-      rewrite ccompose_id_r HEQ.
-      reflexivity.
+    - destruct a.
+      + intros X ? op x y ? s1 s2 k HEQ; simpl.
+        unfold ofe_iso_1'; simpl.
+        rewrite ccompose_id_r HEQ.
+        reflexivity.
+      + intros X ? op x y s1 s2.
+        simpl. eauto.
   Defined.
 
-  #[global] Instance subReifier_there {n} (r r' : sReifier) (rs : gReifiers n) :
+  #[global] Instance subReifier_there {n} {a : is_ctx_dep}
+    (r r' : sReifier a) (rs : gReifiers a n) :
     subReifier r rs →
-    subReifier r (gReifiers_cons r' rs).
+    subReifier r (gReifiers_cons a r' rs).
   Proof.
     intros SR.
     simple refine ({| sR_idx := FS sR_idx |}).
     - simpl. intros. apply sR_state.
-    - intros X ? op x y s1 s2.
-      simpl. apply sR_re.
+    - destruct a.
+      + intros ? X ? op x y s1 s2.
+        simpl. intros.
+        pose proof (@sR_re n CtxDep r rs _ m X _ op) as G.
+        simpl in G.
+        by apply G.
+      + intros ? X ? op x y s1 s2.
+        simpl. intros.
+        pose proof (@sR_re n NotCtxDep r rs _ m X _ op) as G.
+        simpl in G.
+        by apply G.
   Defined.
 
-  #[local] Definition subR_op {n} {r : sReifier} {rs : gReifiers n} `{!subReifier r rs} :
-    opid (sReifier_ops r) → opid (gReifiers_ops rs).
+  #[local] Definition subR_op {n} {a : is_ctx_dep}
+    {r : sReifier a} {rs : gReifiers a n} `{!subReifier r rs} :
+    opid (sReifier_ops a r) → opid (gReifiers_ops a rs).
   Proof.
     intros op.
     simpl.
     refine (existT sR_idx (subEff_opid op)).
   Defined.
-  #[export] Instance subReifier_subEff {n} {r : sReifier} {rs : gReifiers n} `{!subReifier r rs} :
-    subEff (sReifier_ops r) (gReifiers_ops rs).
+
+  #[export] Instance subReifier_subEff {n} {a : is_ctx_dep}
+    {r : sReifier a} {rs : gReifiers a n} `{!subReifier r rs} :
+    subEff (sReifier_ops a r) (gReifiers_ops a rs).
   Proof.
     simple refine {| subEff_opid := subR_op |}.
     - intros op X ?. simpl.
@@ -212,90 +349,216 @@ Section greifiers.
       apply subEff_outs.
   Defined.
 
-  Lemma subReifier_reify_idx {n} (r : sReifier) (rs : gReifiers n)
-    `{!subReifier r rs} {X} `{!Cofe X} (op : opid (sReifier_ops r))
-    (x : Ins (sReifier_ops _ op) ♯ X)
-    (* (y : Outs (sReifier_ops _ op) ♯ X) *)
-    (y : laterO X)
-    (k : (Outs (sReifier_ops r op) ♯ X -n> laterO X))
-    (s1 s2 : sReifier_state r ♯ X) :
-    sReifier_re r op (x, s1, k) ≡ Some (y, s2) →
-      sReifier_re (rs !!! sR_idx) (subEff_opid op)
-        (subEff_ins x, sR_state s1, k ◎ (subEff_outs ^-1)) ≡
-        Some (y, sR_state s2).
+  Program Definition subReifier_reify_idx_type {n}
+    (a : is_ctx_dep) (r : sReifier a) (rs : gReifiers a n)
+    `{!subReifier r rs} X `{!Cofe X} (op : opid (sReifier_ops a r)) : Type.
   Proof.
-    intros Hx. apply equiv_dist=>m.
-    apply sR_re. by apply equiv_dist.
+    destruct a.
+    - apply (∀ (x : Ins (sReifier_ops CtxDep r op) ♯ X)
+               (y : laterO X)
+               (s1 s2 : sReifier_state CtxDep r ♯ X)
+               (k : (Outs (sReifier_ops CtxDep r op) ♯ X -n> laterO X)),
+               sReifier_re CtxDep r op (x, s1, k) ≡ Some (y, s2) →
+               sReifier_re CtxDep (rs !!! sR_idx) (subEff_opid op)
+                 (subEff_ins x, sR_state s1, k ◎ (subEff_outs ^-1)) ≡
+                 Some (y, sR_state s2)).
+    - apply (∀ (x : Ins (sReifier_ops NotCtxDep _ op) ♯ X)
+               (y : Outs (sReifier_ops NotCtxDep _ op) ♯ X)
+               (s1 s2 : sReifier_state NotCtxDep r ♯ X),
+               sReifier_re NotCtxDep r op (x, s1) ≡ Some (y, s2) →
+               sReifier_re NotCtxDep (rs !!! sR_idx) (subEff_opid op)
+                 (subEff_ins x, sR_state s1) ≡
+                 Some (subEff_outs y, sR_state s2)).
+  Defined.
+
+  Lemma subReifier_reify_idx {n} {a : is_ctx_dep}
+    (r : sReifier a) (rs : gReifiers a n)
+    `{!subReifier r rs} {X} `{!Cofe X} (op : opid (sReifier_ops a r))
+    : subReifier_reify_idx_type a r rs X op.
+  Proof.
+    destruct a.
+    - intros Hx. intros. apply equiv_dist=>m.
+      pose proof (@sR_re n CtxDep r rs _ m X _ op Hx y s1 s2 k) as G.
+      simpl in G.
+      rewrite G; first done.
+      by apply equiv_dist.
+    - intros Hx. intros. apply equiv_dist=>m.
+      pose proof (@sR_re n NotCtxDep r rs _ m X _ op Hx y s1 s2) as G.
+      simpl in G.
+      rewrite G; first done.
+      by apply equiv_dist.
   Qed.
 
-  Lemma subReifier_reify {n} (r : sReifier)
-    (rs : gReifiers n) `{!subReifier r rs} {X} `{!Cofe X}
-    (op : opid (sReifier_ops r))
-    (x : Ins (sReifier_ops _ op) ♯ X) (y : laterO X)
-    (k : (Outs (sReifier_ops r op) ♯ X -n> laterO X))
-    (σ σ' : sReifier_state r ♯ X) (rest : gState_rest sR_idx rs ♯ X) :
-    sReifier_re r op (x, σ, k) ≡ Some (y, σ') →
-    gReifiers_re rs (subEff_opid op)
-      (subEff_ins x, gState_recomp rest (sR_state σ), k ◎ (subEff_outs ^-1))
-      ≡ Some (y, gState_recomp rest (sR_state σ')).
+  Program Definition subReifier_reify_type {n} (a : is_ctx_dep) (r : sReifier a)
+    (rs : gReifiers a n) `{!subReifier r rs} X `{!Cofe X}
+    (op : opid (sReifier_ops a r)) : Type.
   Proof.
-    intros Hre.
-    eapply subReifier_reify_idx in Hre.
-    rewrite gReifiers_re_idx//.
-    rewrite Hre. simpl.
-    do 3 f_equiv.
+    destruct a.
+    - apply (∀ (x : Ins (sReifier_ops CtxDep _ op) ♯ X) (y : laterO X)
+               (k : (Outs (sReifier_ops CtxDep r op) ♯ X -n> laterO X))
+               (σ σ' : sReifier_state CtxDep r ♯ X) (rest : gState_rest CtxDep sR_idx rs ♯ X),
+               sReifier_re CtxDep r op (x, σ, k) ≡ Some (y, σ') →
+               gReifiers_re CtxDep rs (subEff_opid op)
+                 (subEff_ins x, gState_recomp CtxDep rest (sR_state σ), k ◎ (subEff_outs ^-1))
+                 ≡ Some (y, gState_recomp CtxDep rest (sR_state σ'))).
+    - apply (∀ (x : Ins (sReifier_ops NotCtxDep _ op) ♯ X) (y : Outs (sReifier_ops NotCtxDep _ op) ♯ X)
+               (σ σ' : sReifier_state NotCtxDep r ♯ X) (rest : gState_rest NotCtxDep sR_idx rs ♯ X),
+               sReifier_re NotCtxDep r op (x,σ) ≡ Some (y, σ') →
+               gReifiers_re NotCtxDep rs (subEff_opid op)
+                 (subEff_ins x, gState_recomp NotCtxDep rest (sR_state σ))
+                 ≡ Some (subEff_outs y, gState_recomp NotCtxDep rest (sR_state σ'))).
+  Defined.
+
+  Lemma subReifier_reify {n} {a : is_ctx_dep} (r : sReifier a)
+    (rs : gReifiers a n) `{!subReifier r rs} {X} `{!Cofe X}
+    (op : opid (sReifier_ops a r)) : subReifier_reify_type a r rs X op.
+  Proof.
+    destruct a.
+    - simpl.
+      intros x y k σ σ' H Hre.
+      pose proof (@subReifier_reify_idx n CtxDep r rs _ X _ op x y σ σ' k Hre) as J; clear Hre.
+      simpl in J.
+      pose proof (@gReifiers_re_idx n CtxDep sR_idx rs X _ (subEff_opid op)) as J'.
+      simpl in J'.
+      rewrite J'; clear J'.
+      transitivity (prod_map (λ x0 : laterO X, x0)
+                      (λ st : sReifier_state CtxDep (rs !!! sR_idx) ♯ X,
+                          (gState_decomp' CtxDep sR_idx rs ^-1) (st, H)) <$>
+                      (Some (y, sR_state σ'))).
+      + unfold prod_map.
+        rewrite option_fmap_proper; [reflexivity | intros ??? | apply J].
+        do 2 f_equiv; first assumption.
+        do 2 f_equiv; assumption.
+      + simpl; reflexivity.
+    - simpl.
+      intros x y σ σ' rest Hre.
+      pose proof (@subReifier_reify_idx n NotCtxDep r rs _ X _ op x y σ σ' Hre)
+        as J; clear Hre.
+      simpl in J.
+      pose proof (@gReifiers_re_idx n NotCtxDep sR_idx rs X _ (subEff_opid op))
+        as J'.
+      simpl in J'.
+      rewrite J'; clear J'.
+      transitivity (prod_map (λ x0 : Outs (sReifier_ops NotCtxDep (rs !!! sR_idx)
+                                             (subEff_opid op)) ♯ X, x0)
+                      (λ st : sReifier_state NotCtxDep (rs !!! sR_idx) ♯ X,
+                          (gState_decomp' NotCtxDep sR_idx rs ^-1) (st, rest)) <$>
+                      (Some (subEff_outs y, sR_state σ'))).
+      + unfold prod_map.
+        rewrite option_fmap_proper; [reflexivity | intros ??? | apply J].
+        do 2 f_equiv; first assumption.
+        do 2 f_equiv; assumption.
+      + simpl; reflexivity.
   Qed.
 
   (** Lemma for reasoning internally in iProp *)
   Context `{!invGS_gen hlc Σ}.
   Notation iProp := (iProp Σ).
   Context {sz : nat}.
-  Variable (rs : gReifiers sz).
-  Notation sr := (gReifiers_sReifier rs).
+  Notation sr a rs := (gReifiers_sReifier a rs).
 
-  Lemma reify_vis_eqI {A} `{!Cofe A} op i k o σ σ' :
-    (gReifiers_re rs op (i, σ, k) ≡ Some (o,σ') ⊢@{iProp} reify sr (Vis op i k : IT _ A) σ ≡ (σ', Tau $ o))%I.
+  Lemma reify_vis_eqI_ctx_dep (rs : gReifiers CtxDep sz)
+    {A} `{!Cofe A} op i k o σ σ' :
+    (gReifiers_re CtxDep rs op (i, σ, k) ≡ Some (o,σ')
+     ⊢@{iProp} reify (sr CtxDep rs) (Vis op i k : IT _ A) σ ≡ (σ', Tau $ o))%I.
   Proof.
     apply uPred.internal_eq_entails=>m.
-    intros H. apply reify_vis_dist. exact H.
+    intros H. apply reify_vis_dist_ctx_dep. exact H.
   Qed.
 
-  Lemma subReifier_reify_idxI (r : sReifier)
-    `{!subReifier r rs} {X} `{!Cofe X} (op : opid (sReifier_ops r))
-    (x : Ins (sReifier_ops _ op) ♯ X)
-    (y : laterO X)
-    (k : (Outs (sReifier_ops r op) ♯ X -n> laterO X))
-    (s1 s2 : sReifier_state r ♯ X) :
-        sReifier_re r op (x, s1, k) ≡ Some (y, s2) ⊢@{iProp}
-        sReifier_re (rs !!! sR_idx) (subEff_opid op)
-          (subEff_ins x, sR_state s1, k ◎ (subEff_outs ^-1)) ≡
-          Some (y, sR_state s2).
+  Lemma reify_vis_eqI_ctx_indep (rs : gReifiers NotCtxDep sz)
+    {A} `{!Cofe A} op i k o σ σ' :
+    (gReifiers_re NotCtxDep rs op (i, σ) ≡ Some (o,σ')
+     ⊢@{iProp} reify (sr NotCtxDep rs) (Vis op i k : IT _ A) σ ≡ (σ', Tau $ k o))%I.
   Proof.
     apply uPred.internal_eq_entails=>m.
-    intros H.
-    rewrite sR_re; last first.
-    - rewrite H.
+    intros H. apply reify_vis_dist_ctx_indep. exact H.
+  Qed.
+
+  Lemma subReifier_reify_idxI_ctx_dep (r : sReifier CtxDep)
+    `{!@subReifier sz CtxDep r rs} {X} `{!Cofe X} (op : opid (sReifier_ops CtxDep r))
+    (x : Ins (sReifier_ops CtxDep _ op) ♯ X)
+    (y : laterO X)
+    (k : (Outs (sReifier_ops CtxDep r op) ♯ X -n> laterO X))
+    (s1 s2 : sReifier_state CtxDep r ♯ X) :
+    sReifier_re CtxDep r op (x, s1, k) ≡ Some (y, s2) ⊢@{iProp}
+                                                         sReifier_re CtxDep (rs !!! sR_idx) (subEff_opid op)
+                                                         (subEff_ins x, sR_state s1, k ◎ (subEff_outs ^-1)) ≡
+                                                         Some (y, sR_state s2).
+  Proof.
+    apply uPred.internal_eq_entails=>m.
+    intros H'.
+    rewrite (sR_re (a := CtxDep)); last first.
+    - rewrite H'.
       reflexivity.
     - reflexivity.
   Qed.
 
-  Lemma subReifier_reifyI (r : sReifier)
-    `{!subReifier r rs} {X} `{!Cofe X}
-    (op : opid (sReifier_ops r))
-    (x : Ins (sReifier_ops _ op) ♯ X) (y : laterO X)
-    (k : (Outs (sReifier_ops r op) ♯ X -n> laterO X))
-    (σ σ' : sReifier_state r ♯ X) (rest : gState_rest sR_idx rs ♯ X) :
-    sReifier_re r op (x,σ, k) ≡ Some (y, σ') ⊢@{iProp}
-    gReifiers_re rs (subEff_opid op)
-      (subEff_ins x, gState_recomp rest (sR_state σ), k ◎ (subEff_outs ^-1))
-      ≡ Some (y, gState_recomp rest (sR_state σ')).
+  Lemma subReifier_reify_idxI_ctx_indep (r : sReifier NotCtxDep)
+    `{!@subReifier sz NotCtxDep r rs} {X} `{!Cofe X} (op : opid (sReifier_ops NotCtxDep r))
+    (x : Ins (sReifier_ops NotCtxDep _ op) ♯ X)
+    (y : Outs (sReifier_ops NotCtxDep _ op) ♯ X)
+    (s1 s2 : sReifier_state NotCtxDep r ♯ X) :
+    sReifier_re NotCtxDep r op (x, s1) ≡ Some (y, s2)
+    ⊢@{iProp}
+       sReifier_re NotCtxDep (rs !!! sR_idx) (subEff_opid op)
+       (subEff_ins x, sR_state s1) ≡
+       Some (subEff_outs y, sR_state s2).
+  Proof.
+    apply uPred.internal_eq_entails=>m.
+    apply (sR_re (a := NotCtxDep)).
+  Qed.
+
+  Lemma subReifier_reifyI_ctx_dep (r : sReifier CtxDep)
+    `{!@subReifier sz CtxDep r rs} {X} `{!Cofe X}
+    (op : opid (sReifier_ops CtxDep r))
+    (x : Ins (sReifier_ops CtxDep _ op) ♯ X) (y : laterO X)
+    (k : (Outs (sReifier_ops CtxDep r op) ♯ X -n> laterO X))
+    (σ σ' : sReifier_state CtxDep r ♯ X) (rest : gState_rest CtxDep sR_idx rs ♯ X) :
+    sReifier_re CtxDep r op (x,σ, k) ≡ Some (y, σ') ⊢@{iProp}
+                                                       gReifiers_re CtxDep rs (subEff_opid op)
+                                                       (subEff_ins x, gState_recomp CtxDep rest (sR_state σ), k ◎ (subEff_outs ^-1))
+                                                       ≡ Some (y, gState_recomp CtxDep rest (sR_state σ')).
   Proof.
     apply uPred.internal_eq_entails=>m.
     intros He.
-    eapply sR_re in He.
-    rewrite gReifiers_re_idx//.
+    eapply (sR_re (a := CtxDep)) in He.
+    rewrite (gReifiers_re_idx CtxDep)//.
     rewrite He. simpl.
     reflexivity.
+  Qed.
+
+  Lemma subReifier_reifyI_ctx_indep (r : sReifier NotCtxDep)
+    `{!@subReifier sz NotCtxDep r rs} {X} `{!Cofe X}
+    (op : opid (sReifier_ops NotCtxDep r))
+    (x : Ins (sReifier_ops NotCtxDep _ op) ♯ X) (y : Outs (sReifier_ops NotCtxDep _ op) ♯ X)
+    (σ σ' : sReifier_state NotCtxDep r ♯ X) (rest : gState_rest NotCtxDep sR_idx rs ♯ X) :
+    sReifier_re NotCtxDep r op (x,σ) ≡ Some (y, σ')
+    ⊢@{iProp}
+       gReifiers_re NotCtxDep rs (subEff_opid op)
+       (subEff_ins x, gState_recomp NotCtxDep rest (sR_state σ))
+       ≡ Some (subEff_outs y, gState_recomp NotCtxDep rest (sR_state σ')).
+  Proof.
+    apply uPred.internal_eq_entails=>m.
+    intros He.
+    eapply (sR_re (a := NotCtxDep)) in He.
+    pose proof (@gReifiers_re_idx sz NotCtxDep sR_idx rs X _ (subEff_opid op)
+                  (subEff_ins x)) as J.
+    simpl in J.
+    simpl.
+    rewrite J//; clear J.
+    transitivity (prod_map (λ x0 : Outs (sReifier_ops NotCtxDep (rs !!! sR_idx)
+                                           (subEff_opid op)) ♯ X, x0)
+                    (λ st : sReifier_state NotCtxDep (rs !!! sR_idx) ♯ X,
+                        (gState_decomp' NotCtxDep sR_idx rs ^-1) (st, rest)) <$>
+                    (Some
+                       (subEff_outs y, sR_state σ'))).
+    - unfold prod_map.
+      rewrite option_fmap_ne; [reflexivity | intros ??? | apply He].
+      do 2 f_equiv; first assumption.
+      do 2 f_equiv; assumption.
+    - simpl.
+      reflexivity.
   Qed.
 
 End greifiers.
